---
title: Grassmann Algebra
author: Keith A. Lewis
institute: KALX, LLC
classoption: fleqn
fleqn: true
abstract: The algebra of space
...

\newcommand\dom{\operatorname{dom}}
\newcommand\cod{\operatorname{cod}}
\renewcommand\ker{\operatorname{ker}}
\newcommand\ran{\operatorname{ran}}
\newcommand\Alg{\operatorname{Alg}}
\newcommand\cat[1]{\mathbf{#1}}
\newcommand\mb[1]{\mathbf{#1}}
\newcommand\RR{\mathbf{R}}
\newcommand\GG{\mathcal{G}}

In the middle of the 19th century Hermann Grassmann came up with a simple
axiom to reduce geometric truth to algebra: the product of two points
is 0 if and only if the points coincide. RenÃ© Descartes demonstrated
how to prove results in Euclidian geometry by associating points in
space with numerical coordinates, but Descartes only considered two and
three dimensions.  Grassmann, living in the tenor of his time, extended
this to any number of dimensions.  He predated Einstien, in one aspect,
by treating all points in space on equal footing.  Grassmann's audaciously
simple notion also predated the modern definition of a vector space. Any
point in space can be chosen as an origin and a vector is just the
difference of a point with the origin.

Grassmann considered the set $E$ of points in a space of any (finite) dimension.
The _Grassmann algebra_ of $E$, $\GG(E)$, is the algebra
generated by the points in $E$ over the real numbers $\RR$ with the axiom $PQ = 0$
if and only if $P = Q$. More precisely, the Grassmann algebra is the quotient algebra
$\GG(E) = \Alg(E)/\Alg(\{PP\mid P\in E\})$.

The algebra over the real numbers generated by any set $S$, $\Alg(S)$, is defined by

- $\RR\subseteq\Alg(S)$
- $S\subseteq\Alg(S)$
- If $a\in\RR$ and $x\in\Alg(S)$ then $ax = xa\in\Alg(S)$
- If $x,y\in\Alg(S)$ then $x + y = y + x$ and $xy$ are in $\Alg(S)$

Note that we do not require $xy = yx$.

__Exercise__. _Show if $x\in\Alg(\{PP\mid P\in E\})$ and $y\in\Alg(S)$
then $xy$ and $yx$ are in $Alg(\{PP\mid P\in E\})$_.

This shows $\Alg(\{PP\mid P\in E\})$ is an ideal of $\Alg(S)$ so the quotient
space is well defined.

__Exercise__. _Prove $PQ = -QP$ for $P,Q\in E$_.

_Hint_: Use $(P + Q)(P + Q) = 0$.

The product $PQ$ represents the oriented one dimensional line segment
from $P$ to $Q$ when $P\not=Q$.
We can interpret $aP + bQ$ as the point
having weight $a + b$ that is the baricenter of $aP$ and $bQ$.

Let $R(t) = P + t(Q - P) = (1 - t)P + tQ$, $t\in R$.
Note $R(t)$ has weight 1, $R(0) = P$, and $R(1) = Q$.

__Exercise__ _Show $PQR(t) = 0$ for $t\in\RR$_.

_Hint_: $PQR(t) = PQ((1 - t)P + tQ)$.

This is an example of incidence involve three points. It means $R(t)$
meets the line determined by $P$ and $Q$ for all $t\in\RR$ if $P\not=Q$.

__Exercise__ _Show $Q - P\not= R(t)$ for any $t\in\RR$_.

Since $R(t)/t = (1/t - 1)P + Q$ and $1/t - 1$ tends to $-1$ as $t$ goes
to infinity, we can think of $Q - P$ as a point at infinity with $0$
weight.  It represents the _vector_ from $P$ to $Q$. We can interpret
$R(t) = P + t(Q - P)$ as the point from $P$ along the vector $Q - P$
with length $t$.

If $PQ = tST$, $t\in\RR$, $P,Q,S,T\in\GG(E)$, we write $PQ/ST = t$.

__Exercise__. _For any $R$ with $PQR = 0$ and $PQ\not=0$ we have $R = (PR/PQ)P + (RQ/PQ)Q$_.

_Hint_: If $R = aP + bQ$ then $PR = bPQ$ and $QR = aQP$.

David Hilbert noticed Euclid's axioms were insufficent to determine when
a point lies between two points. Using Grassman algebra we can define $R$
is between $P$ and $Q$ if and only if $PQR = 0$, $PR/PQ > 0$, and $RQ/PQ
< 1$.

### Example

Three points $P,Q,R\in E$ with $PQR\not=0$ determine a triangle. The
midpoint of the side from $P$ to $Q$ is ${P + Q)/2}$ so
${(P + Q)R/2}$ is the _median_ from $R$ to the midpoint of $P$ and $Q$.
The _centroid_ $(P + Q + R)/3$ lies on the median.

__Exercise__. _Show $(P + Q)R(P + Q + R) = 0$_.

Replacing $P,Q,R$ with $Q,R,P$ and $R,P,Q$ shows all medians of a triange meet at the centroid.

TODO: review

This generalizs to higher dimensions.

## Independence

If $P_0\cdots P_k = tQ_0\cdots Q_k$ for some $t\in\RR$ we write
$P_0\cdots P_k/Q_0\cdots Q_k = t$.

The points $P_0,\ldots,P_k$ are _independent_ if $P_0\cdots P_k\not=0$.

__Lemma__. _If $P_0,\ldots,P_k$ are independent and
$\sum_j a_j P_j = \sum_j b_j P_j$, $a_j,b_j\in\RR$, then $a_i = b_i$ for $0\le i\le k$_.

_Proof_. Multiply both sides by the product of $P_j$ for $0\le j\le k$
except for $j = i$. 
This results in $a_i P_0\cdots P_k = b_i P_0\cdots P_k$
for $0\le i\le k$ using $PP = 0$ for all $P\in\GG(E)$. The result follows from $P_0\cdots P_k/P_0\cdots P_k = 1$.

If $P_0\cdots P_k=0$ we say $P_0,\ldots,P_k$ are _dependent_.

__Lemma__. _If $P_0,\ldots,P_k$ are dependent then there exits $i$ 
and $a_j\in\RR$, $j\not=i$, with
$P_i = \sum_{j\not=i} a_jP_j$_.


This generalizes to any number of dimensions. Let $P_j$ be points in $E$, $0\le j\le n$,
with $P_0\cdots P_n\not=0$. Define $R(t_1,\ldots,t_n)
= (1 - \sum_1^n t_i)P_0 + \sum_1^n t_i P_i$.

__Exercise__. _Show $P_0\cdots P_nR(t_1,\ldots,t_n) = 0$, $t_i\in\RR$_.

__Exercise__. _Show if $P_0\cdots P_nR = 0$ and $P_0\cdots P_n\not=0$ then
$R = \sum_0^n (P_0\cdots R\cdots P_n/P_0\cdots P_n)P_i$ where
$P_i$ is replaced by $R$ in the coefficents of the sum_.

The smallest convex set containing $P_0,\ldots,P_n$
is $\{\sum_i t_i P_i\mid t_i\ge0,\sum_i t_i = 1\}$.
The above exercise show $R$ belongs to the convex hull if and only if
all coefficients in the sum are non-negative.

A finite set of points $P_i\in E$ are _independent_ if $\sum t_i P_i = 0$ implies $t_i = 0$ for all $i$.

__Exercise__. _If $P = \sum_{j = 0}^k t_j P_j$, $t_j\in\RR$, $P_j\in E$ then $P P_0\cdots P_k = 0$_.

_Hint_: $P_j P_0 \cdots P_k = 0$ for all $j$, $1\le j\le k$.

__Exercise__. _Given $P_j\in E$, $0\le j\le k$ and $P P_0\cdots P_k = 0$ then
there exist $t_j\in\RR$ with $P = \sum_{j = 1}^k t_j P_j$_.

The exercises show the _extensor_ $P_0 \cdots P_k \not= 0$ if and only if ${P_0,\ldots, P_k}$ are independent. 
The _order_ of the extensor is the number of points in the product. 

## Progressive Product

If  $A$ and $B$ are extensors with $\langle A\rangle \cap \langle B\rangle = 0$ 
then $\langle A\vee B\rangle = \langle A\rangle \oplus \langle B\rangle$.
If $\langle A\rangle \cap \langle B\rangle \not= 0$ 
then $\langle A\vee B\rangle = 0$.

## Regressive Product

If  $A$ and $B$ are extensors with $\langle A\rangle \cap \langle B\rangle \not= 0$ 
then $\langle A\wedge B\rangle = \langle A\rangle \oplus \langle B\rangle$.
If $\langle A\rangle \cap \langle B\rangle \not= 0$ 
then $\langle A\vee B\rangle = 0$.


The _boundary_ of $PQ$ is $\partial(PQ) = Q - P$.

__Exercise__. _Show $\partial(PQ) = 0$ if and only if $P = Q$_.

